src/kemedhoc/Impl.KEMEDHOC.Ciphertext.fsti
@@ -1,0 +1,190 @@
+module Impl.KEMEDHOC.Ciphertext
+
+(*LowStar related modules*)
+open Lib.ByteBuffer
+open Lib.IntTypes
+open Lib.Buffer
+
+module B = LowStar.Buffer
+module ST = FStar.HyperStack.ST
+module HS = FStar.HyperStack
+module S = FStar.Seq
+module Seq = Lib.Sequence
+
+(*Specification modules*)
+module Spec = Spec.KEMEDHOC.Ciphertext
+module SpecCrypto = Spec.KEMEDHOC.CryptoPrimitives
+
+(*EDHOC utilities*)
+open Impl.EDHOC.Utilities
+
+(*KEMEDHOC utilities*)
+open Impl.KEMEDHOC.Types
+open Impl.KEMEDHOC.CryptoPrimitives
+open Impl.KEMEDHOC.KeySchedule
+open Impl.KEMEDHOC.Parser
+open Spec.KEMEDHOC.Base.Definitions
+
+module TypeEdhoc = TypeHelper.EDHOC
+
+/// -------------
+/// Ciphertext 1
+/// -------------
+val encrypt_plaintext1:
+  #kcs: supportedKemCipherSuite
+  -> ptx1: plaintext1
+  -> th1: hash_out_buff kcs
+  -> prk1e: hash_out_buff kcs
+  -> c1: c1_buff kcs
+  -> ST.Stack c_response
+  (requires fun h0 ->
+    is_valid_plaintext1 h0 ptx1 /\ live h0 th1 /\ live h0 prk1e /\ live h0 c1
+    /\ B.all_disjoint [plaintext1_union ptx1; loc th1; loc prk1e; loc c1]
+  )
+  (ensures fun h0 res h1 ->
+    let c1_s = Spec.encrypt_plaintext1 #kcs (plaintext1_eval h0 ptx1) (as_seq h0 th1) (as_seq h0 prk1e) in
+
+    match res with
+      | TypeEdhoc.CUnsupportedAlgorithmOrInvalidConfig -> modifies0 h0 h1
+      | TypeEdhoc.CSuccess -> (
+        modifies1 c1 h0 h1
+        /\ Seq.equal (as_seq h1 c1) c1_s
+      )
+      | _ -> False
+  )
+
+val decrypt_ciphertext1:
+  #kcs: supportedKemCipherSuite
+  -> c1: c1_buff kcs
+  -> th1: hash_out_buff kcs
+  -> prk1e: hash_out_buff kcs
+  -> ptx1_buffer: plaintext1_buff
+  -> ST.Stack c_response
+  (requires fun h0 ->
+    live h0 c1 /\ live h0 th1 /\ live h0 prk1e /\ live h0 ptx1_buffer
+    /\ B.all_disjoint [loc c1; loc th1; loc prk1e; loc ptx1_buffer]
+  )
+  (ensures fun h0 res h1 ->
+    let ptx1_s_opt = Spec.decrypt_ciphertext1 #kcs (as_seq h0 c1) (as_seq h0 th1) (as_seq h0 prk1e) in
+
+    (match res with
+      | TypeEdhoc.CUnsupportedAlgorithmOrInvalidConfig -> modifies0 h0 h1
+      | TypeEdhoc.CDecryptionFailure -> modifies1 ptx1_buffer h0 h1
+      | TypeEdhoc.CSuccess -> (
+        match ptx1_s_opt with
+          | None -> False
+          | Some ptx1_s ->
+            modifies1 ptx1_buffer h0 h1
+            /\ Seq.equal (as_seq h1 ptx1_buffer) ptx1_s
+      )
+      | _ -> False
+    )
+  )
+
+/// -------------
+/// Ciphertext 2
+/// -------------
+val encrypt_plaintext2:
+  #kcs: supportedKemCipherSuite
+  -> ptx2: plaintext2 kcs
+  -> th2: hash_out_buff kcs
+  -> prk2e: hash_out_buff kcs
+  -> c2: c2_buff kcs
+  -> ST.Stack c_response
+  (requires fun h0 ->
+    is_valid_plaintext2 h0 ptx2 /\ live h0 th2 /\ live h0 prk2e /\ live h0 c2
+    /\ B.all_disjoint [plaintext2_union ptx2; loc th2; loc prk2e; loc c2]
+  )
+  (ensures fun h0 res h1 ->
+    let c2_s = Spec.encrypt_plaintext2 #kcs (plaintext2_eval h0 ptx2) (as_seq h0 th2) (as_seq h0 prk2e) in
+
+    match res with
+      | TypeEdhoc.CUnsupportedAlgorithmOrInvalidConfig -> modifies0 h0 h1
+      | TypeEdhoc.CSuccess -> (
+        modifies1 c2 h0 h1
+        /\ Seq.equal (as_seq h1 c2) c2_s
+      )
+      | _ -> False
+  )
+
+val decrypt_ciphertext2:
+  #kcs: supportedKemCipherSuite
+  -> c2: c2_buff kcs
+  -> th2: hash_out_buff kcs
+  -> prk2e: hash_out_buff kcs
+  -> p2_buffer: plaintext2_buff kcs
+  -> ST.Stack c_response
+  (requires fun h0 ->
+    live h0 c2 /\ live h0 th2 /\ live h0 prk2e /\ live h0 p2_buffer
+    /\ B.all_disjoint [loc c2; loc th2; loc prk2e; loc p2_buffer]
+  )
+  (ensures fun h0 res h1 ->
+    let p2_s_opt = Spec.decrypt_ciphertext2 #kcs (as_seq h0 c2) (as_seq h0 th2) (as_seq h0 prk2e) in
+
+    (match res with
+      | TypeEdhoc.CUnsupportedAlgorithmOrInvalidConfig -> modifies0 h0 h1
+      | TypeEdhoc.CDecryptionFailure -> modifies1 p2_buffer h0 h1
+      | TypeEdhoc.CSuccess -> (
+        match p2_s_opt with
+          | None -> False
+          | Some p2_s ->
+            modifies1 p2_buffer h0 h1
+            /\ Seq.equal (as_seq h1 p2_buffer) p2_s
+      )
+      | _ -> False
+    )
+  )
+
+/// -------------
+/// Ciphertext 3
+/// -------------
+val encrypt_plaintext3:
+  #kcs: supportedKemCipherSuite
+  -> ptx3: plaintext3 kcs
+  -> th3: hash_out_buff kcs
+  -> prk3e2m: hash_out_buff kcs
+  -> c3: c3_buff kcs
+  -> ST.Stack c_response
+  (requires fun h0 ->
+    is_valid_plaintext3 h0 ptx3 /\ live h0 th3 /\ live h0 prk3e2m /\ live h0 c3
+    /\ B.all_disjoint [plaintext3_union ptx3; loc th3; loc prk3e2m; loc c3]
+  )
+  (ensures fun h0 res h1 ->
+    let c3_s = Spec.encrypt_plaintext3 #kcs (plaintext3_eval h0 ptx3) (as_seq h0 th3) (as_seq h0 prk3e2m) in
+
+    match res with
+      | TypeEdhoc.CUnsupportedAlgorithmOrInvalidConfig -> modifies0 h0 h1
+      | TypeEdhoc.CSuccess -> (
+        modifies1 c3 h0 h1
+        /\ Seq.equal (as_seq h1 c3) c3_s
+      )
+      | _ -> False
+  )
+
+val decrypt_ciphertext3:
+  #kcs: supportedKemCipherSuite
+  -> c3: c3_buff kcs
+  -> th3: hash_out_buff kcs
+  -> prk3e2m: hash_out_buff kcs
+  -> p3_buffer: plaintext3_buff kcs
+  -> ST.Stack c_response
+  (requires fun h0 ->
+    live h0 c3 /\ live h0 th3 /\ live h0 prk3e2m /\ live h0 p3_buffer
+    /\ B.all_disjoint [loc c3; loc th3; loc prk3e2m; loc p3_buffer]
+  )
+  (ensures fun h0 res h1 ->
+    let p3_s_opt = Spec.decrypt_ciphertext3 #kcs (as_seq h0 c3) (as_seq h0 th3) (as_seq h0 prk3e2m) in
+
+    (match res with
+      | TypeEdhoc.CUnsupportedAlgorithmOrInvalidConfig -> modifies0 h0 h1
+      | TypeEdhoc.CDecryptionFailure -> modifies1 p3_buffer h0 h1
+      | TypeEdhoc.CSuccess -> (
+        match p3_s_opt with
+          | None -> False
+          | Some p3_s ->
+            modifies1 p3_buffer h0 h1
+            /\ Seq.equal (as_seq h1 p3_buffer) p3_s
+      )
+      | _ -> False
+    )
+  )
